iris/ProofKexecB2.v
@@ -1337,7 +1337,7 @@ Section KexecB2Loops.
                              Hivalid & Hload & #Hity & Hfrz & Hkeep & Hru)".
       iDestruct (kxc_load_peel with "Hload") as
         (datl) "(%Hiok & %Hdok & %Hddix & %Hdoc & %Hduq & Hdlk & Hdiat & Hmeta & Hmap
-               & Hblocks)".
+               & Hblocks & Hdview)".
       pose proof Hiok as Hiok'.
       destruct Hiok' as (Hbmwf & Hbmcov & Hdaddr & Hdty & Hszb & Hholes & Hsized).
       iDestruct (proc_priv_bare_acc gf (proc_addr jp) pidv V with "Hpriv")
@@ -1385,7 +1385,7 @@ Section KexecB2Loops.
       iDestruct ("Hgive" with "Hpage") as "Hpt".
       iDestruct (kxc_load_seal gfs gi cov logstart kf inumf dnf bmf datl
                    Hiok Hdok Hddix Hdoc Hduq
-                   with "Hdlk Hdiat Hmeta Hmap Hblocks") as "Hload".
+                   with "Hdlk Hdiat Hmeta Hmap Hblocks Hdview") as "Hload".
       iDestruct (A.kxa_bs3_join bn with "Hbs1 Hbs2") as "Hbs".
       iDestruct (kxc_open_intro gfs gi cn cov logstart dev pidv kf qf sf gyf
                    inumf dnf bmf gilf gislf
